sail-riscv/test.v
@@ -2,7 +2,7 @@ Require Import Sail.Base.
 Require Import Sail.State_monad.
 Require Import Sail.State_lifting.
 Require Import isla.sail_riscv.sail_opsem.
-From isla.instructions.example Require Import instrs.
+From isla.instructions.riscv64_test Require Import instrs.
 
 (* Eval hnf in riscv.decode (Ox"00a5b533") >>= execute. *)
 (* Eval vm_compute in decodeCompressed (Ox"8526"). *)
@@ -128,7 +128,7 @@ Axiom AXIOM_sim_TakePendingInterrupts : ∀ n Σ i e1 e2,
 (*** reduction tactics *)
 Ltac hnf_sim :=
   match goal with
-  | |- sim _ _ ?e1 _ _ =>
+  | |- sim _ ?e1 _ _ =>
       let e' := eval hnf in e1 in
       change (e1) with e'
   end.
@@ -143,8 +143,32 @@ Ltac reduce_closed_sim :=
    (* | |- context [cast_unit_vec ?b] => progress reduce_closed (cast_unit_vec b) *)
    | |- context [@neq_vec ?n ?b1 ?b2] => progress reduce_closed (@neq_vec n b1 b2)
    | |- context [Z.ltb ?n1 ?n2] => progress reduce_closed (Z.ltb n1 n2)
+   | |- context [Z.leb ?n1 ?n2] => progress reduce_closed (Z.leb n1 n2)
+   | |- context [Z.geb ?n1 ?n2] => progress reduce_closed (Z.geb n1 n2)
    | |- context [Z.eqb ?n1 ?n2] => progress reduce_closed (Z.eqb n1 n2)
    | |- context [neq_int ?n1 ?n2] => progress reduce_closed (neq_int n1 n2)
+   | |- context [size_bits_backwards_matches ?n] => progress reduce_closed (size_bits_backwards_matches n)
+   | |- context [size_bits_backwards ?n] => progress reduce_closed (size_bits_backwards n)
+   | |- context [bool_bits_backwards_matches ?n] => progress reduce_closed (bool_bits_backwards_matches n)
+   | |- context [bool_bits_backwards ?n] => progress reduce_closed (bool_bits_backwards n)
+   | |- context [amo_width_valid ?n] => progress reduce_closed (amo_width_valid n)
+   | |- context [encdec_amoop_backwards_matches ?n] => progress reduce_closed (encdec_amoop_backwards_matches n)
+   | |- context [encdec_amoop_backwards ?n] => progress reduce_closed (encdec_amoop_backwards n)
+   | |- context [encdec_mul_op_backwards_matches ?n] => progress reduce_closed (encdec_mul_op_backwards_matches n)
+   | |- context [encdec_mul_op_backwards ?n] => progress reduce_closed (encdec_mul_op_backwards n)
+   | |- context [bool_not_bits_backwards_matches ?n] => progress reduce_closed (bool_not_bits_backwards_matches n)
+   | |- context [bool_not_bits_backwards ?n] => progress reduce_closed (bool_not_bits_backwards n)
+   | |- context [encdec_csrop_backwards_matches ?n] => progress reduce_closed (encdec_csrop_backwards_matches n)
+   | |- context [encdec_csrop_backwards ?n] => progress reduce_closed (encdec_csrop_backwards n)
+   | |- context [encdec_rounding_mode_backwards_matches ?n] => progress reduce_closed (encdec_rounding_mode_backwards_matches n)
+   | |- context [encdec_rounding_mode_backwards ?n] => progress reduce_closed (encdec_rounding_mode_backwards n)
+(* Decode cannot be reduced for floating point operations. There one has to do something like the following:
+  apply: sim_is_RV32F_or_RV64F => b.
+  red_sim.
+  have -> : (if b then Done false else Done false) = Done false by destruct b.
+  red_sim.
+*)
+   | |- context [riscv.decode ?i] => progress reduce_closed (riscv.decode i)
    | |- context [decodeCompressed ?i] => progress reduce_closed (decodeCompressed i)
    | |- context [get_config_print_reg ()] => progress reduce_closed (get_config_print_reg ())
    (* | |- context [HaveNV2Ext ()] => progress reduce_closed (HaveNV2Ext ()) *)
@@ -154,11 +178,15 @@ Ltac reduce_closed_sim :=
 Ltac cbn_sim :=
   cbn [returnm bind bind0 sim_regs
                (* ProcState_of_regval *)
-               x9_ref x10_ref
-               of_regval read_from write_to regval_from_reg
-       (* PSTATE_ref _PC_ref HCR_EL2_ref SCTLR_EL1_ref SEE_ref __unconditional_ref _R_ref __currentInstr_ref *)
+               x9_ref x10_ref x11_ref misa_ref PC_ref nextPC_ref
+               regval_of of_regval read_from write_to regval_from_reg
+               Misa_of_regval regval_of_Misa
+               ext_control_check_pc
+               (* PSTATE_ref _PC_ref HCR_EL2_ref SCTLR_EL1_ref SEE_ref __unconditional_ref _R_ref __currentInstr_ref *)
+               bitU_of_bool bool_of_bitU bit_to_bool
        negb sumbool_of_bool set
-       projT1 __id andb orb
+       projT1 build_ex __id andb orb
+       _rec_execute compressed_measure Zwf_guarded
        subst_val_event subst_val_valu subst_val_smt subst_val_exp subst_val_base_val fmap list_fmap eq_var_name Z.eqb Pos.eqb map
     ].
 
@@ -172,12 +200,22 @@ Ltac red_monad_sim :=
          | |- sim _ (_ >>= _) _ _  => apply sim_bind
          | |- sim _ (_ >> _) _ _  => apply sim_bind
          | |- sim _ (and_boolM _ _) _ _  => apply sim_bind
+         | |- sim _ (and_boolMP _ _) _ _  => apply sim_bind
+         | |- sim _ (projT1_m _) _ _  => apply sim_bind
+         | |- sim _ (build_trivial_ex _) _ _  => apply sim_bind
          | |- sim _ (try_catch _ _) _ _  => apply sim_try_catch
          | |- sim _ (Done _) (BindMCtx _ _) _  => apply sim_pop_bind_Done
          | |- sim _ (Done _) (TryMCtx _ _) _  => apply sim_pop_try_Done
+         | |- sim _ (assert_exp' _ _) _ _  => apply sim_assert_exp';
+              [try done; shelve| let H := fresh in move => H; try clear H]
          | |- sim _ _ _ (Smt (DeclareConst _ (Ty_BitVec _)) _::_)  => apply: sim_DeclareConstBitVec
          | |- sim _ _ _ (Smt (DefineConst _ _) _::_)  => apply: sim_DefineConst; [simpl; done|]
+         | |- sim _ _ _ (Smt (Assert _) _::_)  => apply: sim_Assert; [simpl; shelve|]
+         | |- sim _ _ _ (Branch _ _ _::_)  => apply: sim_Branch
+         | |- sim _ _ _ (Assume _ _::_)  => let H := fresh "Hassume" in apply: sim_Assume => H; simpl in H
          | |- sim _ (read_reg _) _ (ReadReg _ _ _ _::_)  => apply: sim_read_reg; [done | done | try done; shelve|]
+         | |- sim _ (write_reg nextPC_ref _) _ _  => apply: sim_write_reg_private; [done..|]
+         | |- sim _ (read_reg nextPC_ref) _ _  => apply: sim_read_reg_l; [done..|]
          | |- sim _ (write_reg _ _) _ (WriteReg _ _ _ _::_)  => apply: sim_write_reg; [done | shelve |]
          | |- sim _ (Done _) NilMCtx []  => apply: sim_done
          end.
@@ -194,12 +232,124 @@ Ltac red_sim :=
         progress red_monad_sim
       ].
 
+Lemma sim_haveFExt Σ K e2:
+  (∀ b, sim Σ (Done b) K e2) →
+  sim Σ (haveFExt ()) K e2.
+Proof.
+  move => Hsim.
+  unfold haveFExt. red_sim.
+  apply: sim_read_reg_l; [done|]. red_sim.
+  case_match => //. red_sim.
+  apply: sim_read_reg_l; [done|].
+  by red_sim.
+Qed.
+
+Lemma sim_is_RV32F_or_RV64F Σ K e2:
+  (∀ b, sim Σ (Done b) K e2) →
+  sim Σ (is_RV32F_or_RV64F ()) K e2.
+Proof.
+  move => Hsim.
+  unfold is_RV32F_or_RV64F. red_sim.
+  apply: sim_haveFExt => -[]; by red_sim.
+Qed.
+
+Lemma sim_is_RV64F Σ K e2:
+  (∀ b, sim Σ (Done b) K e2) →
+  sim Σ (is_RV64F ()) K e2.
+Proof.
+  move => Hsim.
+  unfold is_RV64F. red_sim.
+  apply: sim_haveFExt => -[]; by red_sim.
+Qed.
+
+Lemma sim_haveDExt Σ K e2:
+  (∀ b, sim Σ (Done b) K e2) →
+  sim Σ (haveDExt ()) K e2.
+Proof.
+  move => Hsim.
+  unfold haveDExt. red_sim.
+  apply: sim_read_reg_l; [done|]. red_sim.
+  case_match => //. red_sim.
+  apply: sim_read_reg_l; [done|].
+  by red_sim.
+Qed.
+
+Lemma sim_is_RV32D_or_RV64D Σ K e2:
+  (∀ b, sim Σ (Done b) K e2) →
+  sim Σ (is_RV32D_or_RV64D ()) K e2.
+Proof.
+  move => Hsim.
+  unfold is_RV32D_or_RV64D. red_sim.
+  apply: sim_haveDExt => -[]; by red_sim.
+Qed.
+
+Lemma sim_is_RV64D Σ K e2:
+  (∀ b, sim Σ (Done b) K e2) →
+  sim Σ (is_RV64D ()) K e2.
+Proof.
+  move => Hsim.
+  unfold is_RV64D. red_sim.
+  apply: sim_haveDExt => -[]; by red_sim.
+Qed.
+
 Lemma sim_instr_mv_a1_s1:
   sim_instr (Compressed [BV{16} 0x85a6]) mv_a1_s1_trace.
 Proof.
   move => regs. eexists _. split; [by left|].
-  unfold step_cpu. red_sim. unfold execute => /=.
+  unfold step_cpu. red_sim. unfold execute. red_sim.
   unfold execute_RTYPE. red_sim.
+Admitted.
+  (* Unshelve. *)
+  (* - simpl. rewrite mword_to_bv_add_vec //. *)
+(* Qed. *)
+
+
+Lemma sim_instr_a0:
+  sim_instr (Uncompressed [BV{32} 0x00000513]) a0.
+Proof.
+  move => regs. eexists _. split; [by left|].
+  unfold step_cpu. red_sim. unfold execute. red_sim.
+  unfold execute_ITYPE. red_sim.
   Unshelve.
-  - simpl. rewrite mword_to_bv_add_vec //.
+  all: try done.
+  - simpl. destruct regs => /=. rewrite mword_to_bv_add_vec //.
 Qed.
+
+Lemma sim_instr_a4:
+  sim_instr (Uncompressed [BV{32} 0x00150513]) a4.
+Proof.
+  move => regs. eexists _. split; [by left|].
+  unfold step_cpu. red_sim. unfold execute. red_sim.
+  unfold execute_ITYPE. red_sim.
+  Unshelve.
+  all: try done.
+  - simpl. destruct regs => /=. rewrite mword_to_bv_add_vec //.
+  - simpl. destruct regs => /=. rewrite mword_to_bv_add_vec //.
+Qed.
+
+Lemma sim_instr_a8:
+  sim_instr (Uncompressed [BV{32} 0x00b50463]) a8.
+Proof.
+  move => regs.
+  destruct (eq_vec (x10 regs) (x11 regs)) eqn: Hb1.
+  all: eexists _; split; [by left|].
+  all: unfold step_cpu; red_sim; unfold execute; red_sim.
+  all: unfold execute_BTYPE; red_sim.
+  all: apply: sim_read_reg_l; [done|]; red_sim.
+Admitted.
+(*
+
+  rewrite Hb1; red_sim.
+  unfold access_vec_dec, access_mword_dec.
+  match goal with
+  | |- context [getBit ?w ?n] => destruct (getBit w n) eqn:Hbit
+  end.
+  all: red_sim.
+  all: admit.
+  Unshelve.
+  all: try done.
+  - admit.
+  - admit.
+  - simpl. rewrite mword_to_bv_add_vec //.
+Admitted.
+*)
